Cleanup M

M.lean
@@ -1,17 +1,19 @@
+def Eq.revRec {α : Sort u} {a : α} {motive : ∀ b, a = b → Sort v} {b} h (m : motive b h) : motive a rfl :=
+  h.symm.rec (motive := fun a' h' => motive a' (h.trans h')) m
+
 namespace M
 
 variable {α : Type u} (β : (a : α) → Type v)
 
-private inductive Approx : (ℓ : Nat) → Type (max u v)
-  | hole : Approx .zero
-  | node a (t : (b : β a) → Approx ℓ) : Approx ℓ.succ
+private def Approx : (ℓ : Nat) → Type (max u v)
+  | .zero => PUnit
+  | .succ ℓ => Σ a, (b : β a) → Approx ℓ
 
 variable {β}
 
-private inductive Approx.Agree : (m : Approx β ℓ) → (m' : Approx β ℓ') → Prop
-  | hole {m' : Approx β ℓ'} : Agree hole m'
-  | hole' {m : Approx β ℓ} : Agree m hole
-  | node a {t : (b : β a) → Approx β ℓ} {t' : (b : β a) → Approx β ℓ'} (h : ∀ b, Agree (t b) (t' b)) : Agree (node a t) (node a t')
+private def Approx.Agree : ∀ {ℓ ℓ'}, (m : Approx β ℓ) → (m' : Approx β ℓ') → Prop
+  | .zero, _, _, _ | .succ _, .zero, _, _ => True
+  | .succ _, .succ _, a, a' => ∃ h : a.fst = a'.fst, ∀ b, Approx.Agree (a.snd b) (a'.snd (h ▸ b))
 
 end M
 
@@ -27,73 +29,62 @@ variable {α : Type u} {β : (a : α) → Type v}
 
 @[irreducible]
 def hd (m : M β) : α :=
-  let .node a _ := m.val (.succ .zero)
-  a
+  (m.val (.succ .zero)).fst
 
 unseal hd
 
-private theorem hd_eq {m : M β} (h : m.val (.succ ℓ) = .node a t) : hd m = a := by
-  dsimp only [hd]
-  split
-  next h' =>
-  cases h ▸ h' ▸ m.property (.succ .zero) ℓ.succ
-  rfl
+private theorem hd_eq {m : M β} (h : m.val (.succ ℓ) = ⟨a, t⟩) : hd m = a :=
+  (h ▸ (m.property (.succ .zero) ℓ.succ).1 :)
 
 @[irreducible]
 def tl (m : M β) (b : β m.hd) : M β where
-  val ℓ := match h : m.val ℓ.succ with | .node _ t => t (hd_eq h ▸ b)
-  property ℓ ℓ' := by dsimp only; split; split; next h _ _ h' => cases h ▸ h' ▸ m.property ℓ.succ ℓ'.succ with | node _ h => apply h
+  val ℓ := (m.val ℓ.succ).snd (hd_eq rfl ▸ b)
+  property ℓ ℓ' := by have := (m.property ℓ.succ ℓ'.succ).2 (hd_eq rfl ▸ b); grind only
 
 unseal tl
 
-private theorem tl_eq {m : M β} {t} (h : m.val (.succ ℓ) = .node a t) b : (tl m (hd_eq h ▸ b)).val ℓ = t b := by
-  cases hd_eq h
+private theorem tl_eq {m : M β} (h : m.val (.succ ℓ) = ⟨a, t⟩) b : (tl m (hd_eq h ▸ b)).val ℓ = t b := by
+  obtain ⟨rfl, ⟨⟩⟩ := Sigma.ext_iff.mp h
   dsimp only [tl]
-  split
-  next h' =>
-  cases h ▸ h'
-  rfl
+  grind only
 
 theorem ext {r : (m m' : M β) → Prop} (hd : ∀ {m m'}, (h : r m m') → m.hd = m'.hd) (tl : ∀ {m m'} h b, r (tl m b) (tl m' (hd h ▸ b))) {m m'} (h : r m m') : m = m' := by
   apply Subtype.eq
   funext ℓ
-  induction ℓ using Nat.rec generalizing m m' with
-  | zero =>
-    cases m.val .zero
-    cases m'.val .zero
-    rfl
+  induction ℓ generalizing m m' with
+  | zero => rfl
   | succ ℓ ih =>
     cases h₁ : m.val ℓ.succ
     cases hd_eq h₁
     cases h₂ : m'.val ℓ.succ
-    cases hd_eq h₂ ▸ hd h
+    cases (hd h).trans (hd_eq h₂)
     exact congrArg _ <| funext fun b => tl_eq h₁ b ▸ tl_eq h₂ b ▸ ih (tl h b)
 
 variable {C : Sort w} (hd : (c : C) → α) (tl : ∀ c, (b : β (hd c)) → C) (c : C)
 
 @[irreducible]
-def gen : M β where
-  val ℓ := ℓ.rec (fun _ => .hole) (fun _ gen c => .node (hd c) fun b => gen (tl c b)) c
-  property ℓ := ℓ.rec (fun _ _ => .hole) (fun _ gen c ℓ' => ℓ'.casesOn .hole' fun ℓ' => .node (hd c) fun b => gen (tl c b) ℓ') c
+def corec : M β where
+  val ℓ := ℓ.rec (fun _ => ⟨⟩) (fun _ corec c => ⟨hd c, fun b => corec (tl c b)⟩) c
+  property ℓ := ℓ.rec (fun _ _ => ⟨⟩) (fun _ corec c ℓ' => ℓ'.casesOn ⟨⟩ fun ℓ' => ⟨rfl, fun b => corec (tl c b) ℓ'⟩) c
 
-unseal gen
-
-@[simp]
-theorem hd_gen : (gen hd tl c).hd = hd c := rfl
+unseal corec
 
 @[simp]
-theorem tl_gen : (gen hd tl c).tl b = gen hd tl (tl c b) := rfl
+theorem hd_corec : (corec hd tl c).hd = hd c := rfl
 
-unif_hint {rhs : α} where hd c ≟ rhs ⊢ (gen hd tl c).hd ≟ rhs
-unif_hint {b : β (gen hd tl c).hd} {rhs : M β} where gen hd tl (tl c b) ≟ rhs ⊢ (gen hd tl c).tl b ≟ rhs
-unif_hint {b : β (hd c)} {rhs : M β} where gen hd tl (tl c b) ≟ rhs ⊢ (gen hd tl c).tl b ≟ rhs
+@[simp]
+theorem tl_corec : (corec hd tl c).tl b = corec hd tl (tl c b) := rfl
+
+unif_hint {rhs : α} where hd c ≟ rhs ⊢ (corec hd tl c).hd ≟ rhs
+unif_hint {b : β (corec hd tl c).hd} {rhs : M β} where corec hd tl (tl c b) ≟ rhs ⊢ (corec hd tl c).tl b ≟ rhs
+unif_hint {b : β (hd c)} {rhs : M β} where corec hd tl (tl c b) ≟ rhs ⊢ (corec hd tl c).tl b ≟ rhs
 
 variable (hd : α) (tl : (b : β hd) → M β)
 
 @[irreducible]
 def mk : M β where
-  val ℓ := ℓ.casesOn .hole fun ℓ => .node hd fun b => (tl b).val ℓ
-  property ℓ ℓ' := ℓ.casesOn .hole fun ℓ => ℓ'.casesOn .hole' fun ℓ' => .node hd fun b => (tl b).property ℓ ℓ'
+  val ℓ := ℓ.casesOn ⟨⟩ fun ℓ => ⟨hd, fun b => (tl b).val ℓ⟩
+  property ℓ ℓ' := ℓ.casesOn ⟨⟩ fun ℓ => ℓ'.casesOn ⟨⟩ fun ℓ' => ⟨rfl, fun b => (tl b).property ℓ ℓ'⟩
 
 unseal mk
 
@@ -114,16 +105,15 @@ namespace IM
 
 variable {ι : Type u} {α : (i : ι) → Type v} {β : ∀ i, (a : α i) → Type w} (s : ∀ i a, (b : β i a) → ι)
 
-private inductive Approx : (i : ι) → (ℓ : Nat) → Type (max u v w)
-  | hole : Approx i .zero
-  | node a (t : ∀ b, Approx (s i a b) ℓ) : Approx i ℓ.succ
+private def Approx (i : ι) : (ℓ : Nat) → Type (max u v w)
+  | .zero => PUnit
+  | .succ ℓ => Σ a, ∀ b, Approx (s i a b) ℓ
 
 variable {s}
 
-private inductive Approx.Agree : (m : Approx s i ℓ) → (m' : Approx s i ℓ') → Prop
-  | hole {m' : Approx s i ℓ'} : Agree hole m'
-  | hole' {m : Approx s i ℓ} : Agree m hole
-  | node a {t : ∀ b, Approx s (s i a b) ℓ} {t' : ∀ b, Approx s (s i a b) ℓ'} (h : ∀ b, Agree (t b) (t' b)) : Agree (node a t) (node a t')
+private def Approx.Agree : ∀ {ℓ ℓ'}, (m : Approx s i ℓ) → (m' : Approx s i ℓ') → Prop
+  | .zero, _, _, _ | .succ _, .zero, _, _ => True
+  | .succ _, .succ ℓ', a, a' => ∃ h : a.fst = a'.fst, ∀ b, Approx.Agree (a.snd b) (h.revRec (motive := fun a h => Approx s (s i a (h ▸ b)) ℓ') (a'.snd (h ▸ b)))
 
 end IM
 
@@ -139,82 +129,66 @@ variable {ι : Type u} {α : (i : ι) → Type v} {β : ∀ i, (a : α i) → Ty
 
 @[irreducible]
 def hd (m : IM s i) : α i :=
-  let .node a _ := m.val (.succ .zero)
-  a
+  (m.val (.succ .zero)).fst
 
 unseal hd
 
-private theorem hd_eq {m : IM s i} (h : m.val (.succ ℓ) = .node a t) : hd m = a := by
-  dsimp only [hd]
-  split
-  next h' =>
-  cases h ▸ h' ▸ m.property (.succ .zero) ℓ.succ
-  rfl
+private theorem hd_eq {m : IM s i} (h : m.val (.succ ℓ) = ⟨a, t⟩) : hd m = a :=
+  (h ▸ (m.property (.succ .zero) ℓ.succ).1 :)
 
 @[irreducible]
 def tl (m : IM s i) (b : β i m.hd) : IM s (s i m.hd b) where
-  val ℓ := match h : m.val ℓ.succ with | .node _ t => by cases hd_eq h; exact t b
-  property ℓ ℓ' := by dsimp only; split; split; next h _ _ h' => cases hd_eq h; cases h ▸ h' ▸ m.property ℓ.succ ℓ'.succ with | node _ h => apply h
-
-def tl' (m : IM s i) (h : a = m.hd) : (b : β i a) → IM s (s i a b) := by
-  cases h
-  exact m.tl
+  val ℓ := (hd_eq rfl).revRec (motive := fun a h => Approx s (s i a (h ▸ b)) ℓ) ((m.val ℓ.succ).snd (hd_eq rfl ▸ b))
+  property ℓ ℓ' := by have := (m.property ℓ.succ ℓ'.succ).2 (hd_eq rfl ▸ b); grind only [Eq.revRec]
 
 unseal tl
 
-private theorem tl_eq {m : IM s i} {t} (h : m.val (.succ ℓ) = .node m.hd t) b : (tl m b).val ℓ = t b := by
-  dsimp only [tl]
-  split
-  next h' =>
-  cases h ▸ h'
-  rfl
-
-private theorem tl'_eq {m : IM s i} {t} (h : m.val (.succ ℓ) = .node a t) b : (tl' m (hd_eq h).symm b).val ℓ = t b := by
+private theorem tl_eq {m : IM s i} (h : m.val (.succ ℓ) = ⟨a, t⟩) b : ((hd_eq h).symm.revRec (motive := fun a h => IM s (s i a (h ▸ b))) (tl m (hd_eq h ▸ b))).val ℓ = t b := by
+  have : (congrArg Sigma.fst h).symm.revRec (motive := fun a h => Approx s (s i a (h ▸ b)) ℓ) ((m.val ℓ.succ).snd (congrArg Sigma.fst h ▸ b)) = t b := by
+    obtain ⟨rfl, ⟨⟩⟩ := Sigma.ext_iff.mp h
+    rfl
   cases hd_eq h
-  exact tl_eq h b
+  exact this
 
-theorem ext {r : ∀ i, (m m' : IM s i) → Prop} (hd : ∀ {i m m'}, (h : r i m m') → m.hd = m'.hd) (tl : ∀ {i m m'} (h : r i m m') b, r (s i m.hd b) (tl m b) (tl' m' (hd h) b)) {i m m'} (h : r i m m') : m = m' := by
+theorem ext {r : ∀ i, (m m' : IM s i) → Prop} (hd : ∀ {i m m'}, (h : r i m m') → m.hd = m'.hd) (tl : ∀ {i m m'} (h : r i m m') b, r (s i m.hd b) (tl m b) ((hd h).revRec (motive := fun a h => IM s (s i a (h ▸ b))) (tl m' (hd h ▸ b)))) {i m m'} (h : r i m m') : m = m' := by
   apply Subtype.eq
   funext ℓ
-  induction ℓ using Nat.rec generalizing i with
-  | zero =>
-    cases m.val .zero
-    cases m'.val .zero
-    rfl
+  induction ℓ generalizing i with
+  | zero => rfl
   | succ ℓ ih =>
     cases h₁ : m.val ℓ.succ
     cases hd_eq h₁
     cases h₂ : m'.val ℓ.succ
-    cases hd_eq h₂ ▸ hd h
-    exact congrArg _ <| funext fun b => tl_eq h₁ b ▸ tl'_eq h₂ b ▸ ih (tl h b)
+    cases (hd h).trans (hd_eq h₂)
+    exact congrArg _ <| funext fun b => tl_eq h₁ b ▸ tl_eq h₂ b ▸ ih (tl h b)
 
 variable {C : (i : ι) → Sort x} (hd : ∀ {i}, (c : C i) → α i) (tl : ∀ {i} c, (b : β i (hd c)) → C (s i (hd c) b)) {i} (c : C i)
 
 @[irreducible]
-def gen : IM s i where
-  val ℓ := ℓ.rec (fun _ _ => .hole) (fun _ gen i c => .node (hd c) fun b => gen (s i (hd c) b) (tl c b)) i c
-  property ℓ := ℓ.rec (fun _ _ _ => .hole) (fun _ gen i c ℓ' => ℓ'.casesOn .hole' fun ℓ' => .node (hd c) fun b => gen (s i (hd c) b) (tl c b) ℓ') i c
+def corec : IM s i where
+  val ℓ := ℓ.rec (fun _ _ => ⟨⟩) (fun _ corec i c => ⟨hd c, fun b => corec (s i (hd c) b) (tl c b)⟩) i c
+  property ℓ := ℓ.rec (fun _ _ _ => ⟨⟩) (fun _ corec i c ℓ' => ℓ'.casesOn ⟨⟩ fun ℓ' => ⟨rfl, fun b => corec (s i (hd c) b) (tl c b) ℓ'⟩) i c
 
-unseal gen
-
-@[simp]
-theorem hd_gen : (gen @hd @tl c).hd = hd c := rfl
+unseal corec
 
 @[simp]
-theorem tl_gen : (gen @hd @tl c).tl b = gen @hd @tl (tl c b) := rfl
+theorem hd_corec : (corec @hd @tl c).hd = hd c := rfl
 
-unif_hint {rhs : α i} where hd c ≟ rhs ⊢ (gen @hd @tl c).hd ≟ rhs
-unif_hint {b : β i (gen @hd @tl c).hd} {rhs : IM s (s i (gen @hd @tl c).hd b)} where gen @hd @tl (tl c b) ≟ rhs ⊢ (gen @hd @tl c).tl b ≟ rhs
-unif_hint {b : β i (gen @hd @tl c).hd} {rhs : IM s (s i (hd c) b)} where gen @hd @tl (tl c b) ≟ rhs ⊢ (gen @hd @tl c).tl b ≟ rhs
-unif_hint {b : β i (hd c)} {rhs : IM s (s i (gen @hd @tl c).hd b)} where gen @hd @tl (tl c b) ≟ rhs ⊢ (gen @hd @tl c).tl b ≟ rhs
-unif_hint {b : β i (hd c)} {rhs : IM s (s i (hd c) b)} where gen @hd @tl (tl c b) ≟ rhs ⊢ (gen @hd @tl c).tl b ≟ rhs
+@[simp]
+theorem tl_corec : (corec @hd @tl c).tl b = corec @hd @tl (tl c b) := rfl
+
+unif_hint {rhs : α i} where hd c ≟ rhs ⊢ (corec @hd @tl c).hd ≟ rhs
+unif_hint {b : β i (corec @hd @tl c).hd} {rhs : IM s (s i (corec @hd @tl c).hd b)} where corec @hd @tl (tl c b) ≟ rhs ⊢ (corec @hd @tl c).tl b ≟ rhs
+unif_hint {b : β i (corec @hd @tl c).hd} {rhs : IM s (s i (hd c) b)} where corec @hd @tl (tl c b) ≟ rhs ⊢ (corec @hd @tl c).tl b ≟ rhs
+unif_hint {b : β i (hd c)} {rhs : IM s (s i (corec @hd @tl c).hd b)} where corec @hd @tl (tl c b) ≟ rhs ⊢ (corec @hd @tl c).tl b ≟ rhs
+unif_hint {b : β i (hd c)} {rhs : IM s (s i (hd c) b)} where corec @hd @tl (tl c b) ≟ rhs ⊢ (corec @hd @tl c).tl b ≟ rhs
 
 variable (hd : α i) (tl : (b : β i hd) → IM s (s i hd b))
 
 @[irreducible]
 def mk : IM s i where
-  val ℓ := ℓ.casesOn .hole fun ℓ => .node hd fun b => (tl b).val ℓ
-  property ℓ ℓ' := ℓ.casesOn .hole fun ℓ => ℓ'.casesOn .hole' fun ℓ' => .node hd fun b => (tl b).property ℓ ℓ'
+  val ℓ := ℓ.casesOn ⟨⟩ fun ℓ => ⟨hd, fun b => (tl b).val ℓ⟩
+  property ℓ ℓ' := ℓ.casesOn ⟨⟩ fun ℓ => ℓ'.casesOn ⟨⟩ fun ℓ' => ⟨rfl, fun b => (tl b).property ℓ ℓ'⟩
 
 unseal mk
 
